cfrontend/BeePL_typesystem.v
@@ -5,7 +5,7 @@ Require Import Csyntax Csem SimplExpr Ctypes Memtype.
 Require Import BeePL_aux BeePL_mem BeeTypes BeePL BeePL_auxlemmas Errors BeePL_values.
 From mathcomp Require Import all_ssreflect. 
 
-Definition empty_effect : effect := nil. 
+(*Definition empty_effect : effect := nil. 
 
 Inductive type_expr : ty_context -> store_context -> expr -> effect -> type -> Prop :=
 (*For all value expression, we can assume any effect type, including the empty effect *)
@@ -602,4 +602,4 @@ Lemma well_typed_success:
 Proof.
 apply type_exprs_type_expr_ind_mut=> //=.
 Admitted.*)
-
+*)
