compiler_test/beepl_test/BeePL_progs.v
@@ -3,9 +3,9 @@ Require Import AST Maps Ctypes.
 Require Import BeePL BeeTypes Errors BeePL_typechecker Csyntaxdefs BeePL_Option_Struct. 
 From Coq Require Import String.
 
-Require Import BeePL_add BeePL_cond BeePL_app BeePL_div_zero BeePL_div_zero1 BeePL_external_call BeePL_ref.
-Require Import BeePL_struct_ex2 BeePL_for_ex1 BeePL_for_ex2.
-Require Import BeePL_bpf_get_prandom. (*BeePL_null_ptr BeePL_match_fail_ex1.*)
+Require Import BeePL_add. (* BeePL_cond BeePL_app BeePL_div_zero BeePL_div_zero1 BeePL_external_call BeePL_ref.
+Require Import BeePL_struct_ex2 BeePL_for_ex1 BeePL_for_ex2 BeePL_globvar1.
+Require Import BeePL_bpf_get_prandom BeePL_bpf_ktime_get_ns.*) (*BeePL_null_ptr BeePL_match_fail_ex1.*)
 
 (* In this file you will see two definitions. One for example1 and the other for
    example1_atom_of_string. Those two definitions are extracted to OCaml by 
